examples/dsls/mini_steel/Pulse.Checker.Inference.fsti
@@ -4,5 +4,10 @@ open Pulse.Syntax
 
 module T = FStar.Tactics
 
+val try_inst_uvs_in_goal (uvs:list term)
+                         (ctxt:term)
+                         (goal:vprop)
+  : T.Tac (list (term & term))
+
 val infer (head:term) (t_head:term) (ctxt_pre:term)
   : T.Tac st_term
